The Friendly Character!

Phi_Logic_Programming_Reasoner/PLPR_error_msg.thy
@@ -13,11 +13,18 @@ section \<open>Error Reporting\<close>
 subsection \<open>Encoding of Text\<close>
 
 typedecl "text"
-consts literal_text :: \<open>(text \<Rightarrow> text) \<Rightarrow> text\<close>
-       term_text :: \<open>'a::{} \<Rightarrow> text\<close>
-       type_text :: \<open>'a::{} itself \<Rightarrow> text\<close>
-       cat_text :: \<open>text \<Rightarrow> text \<Rightarrow> text\<close>
-      "text" :: \<open>text \<Rightarrow> text\<close>
+
+setup \<open>Sign.mandatory_path "text"\<close>
+
+consts literal :: \<open>(text \<Rightarrow> text) \<Rightarrow> text\<close>
+       "term"  :: \<open>'a::{} \<Rightarrow> text\<close>
+       type    :: \<open>'a::{} itself \<Rightarrow> text\<close>
+       cat     :: \<open>text \<Rightarrow> text \<Rightarrow> text\<close>
+       newline :: \<open>text\<close>
+      "text"    :: \<open>text \<Rightarrow> text\<close>
+
+setup \<open>Sign.parent_path\<close>
+
 text \<open>We use the name of a lambda variable to encode an arbitrary string text.\<close>
 
 nonterminal "text_"
@@ -25,12 +32,11 @@ syntax "_text_" :: \<open>text_ \<Rightarrow> text\<close> ("TEXT'(_')" [1] 1000
 syntax "_text_literal_" :: \<open>cartouche \<Rightarrow> text_\<close> ("_")
 syntax "_text_term_" :: \<open>logic \<Rightarrow> text_\<close> ("_" [1000] 999)
 syntax "_text_prop_" :: \<open>prop \<Rightarrow> text_\<close> ("_" [1000] 999)
+syntax "_text_newline_" :: \<open>text_\<close> ("\<newline>")
 syntax "_text_cat_" :: \<open>text_ \<Rightarrow> text_ \<Rightarrow> text_\<close> ("_ _" [1,2] 1)
 
-declare [[ML_debugger]]
-
 ML \<open>
-structure Encode_Text = struct
+structure Text_Encoding = struct
 
 val escape_string   = String.translate (fn #"." => "\001" | x => str x)
 val recovery_string = String.translate (fn #"\001" => "." | x => str x)
@@ -40,30 +46,33 @@ local open Ast
     | dest_literal (Appl [Constant \<^syntax_const>\<open>_bound\<close>, x]) = dest_literal x
     | dest_literal (Variable x) = recovery_string x
 
-fun decode_text_ast' ret (Appl [Constant \<^const_syntax>\<open>literal_text\<close>,
+fun decode_text_ast' ret (Appl [Constant \<^const_syntax>\<open>text.literal\<close>,
       Appl [Constant \<^syntax_const>\<open>_abs\<close>, x, _]])
       = Variable (cartouche (dest_literal x))::ret
-  | decode_text_ast' ret (Appl [Constant \<^const_syntax>\<open>term_text\<close>, tm])
+  | decode_text_ast' ret (Appl [Constant \<^const_syntax>\<open>text.term\<close>, tm])
       = tm::ret
-  | decode_text_ast' ret (Appl [Constant \<^const_syntax>\<open>type_text\<close>, tm])
+  | decode_text_ast' ret (Appl [Constant \<^const_syntax>\<open>text.type\<close>, tm])
       = tm::ret
-  | decode_text_ast' ret (Appl [Constant \<^const_syntax>\<open>cat_text\<close>, tmA, tmB])
+  | decode_text_ast' ret (Constant \<^const_syntax>\<open>text.newline\<close>)
+      = (Constant \<^syntax_const>\<open>_text_newline_\<close>)::ret
+  | decode_text_ast' ret (Appl [Constant \<^const_syntax>\<open>text.cat\<close>, tmA, tmB])
       = decode_text_ast' (decode_text_ast' ret tmB) tmA
   | decode_text_ast' _ ast = raise AST ("decode_text_ast", [ast])
 
 in
 
-fun decode_text _ (\<^const>\<open>literal_text\<close> $ Abs (text, _, _)) = [Pretty.str (recovery_string text)]
-  | decode_text ctxt (Const (\<^const_name>\<open>term_text\<close>, _) $ x) = [Syntax.pretty_term ctxt x]
-  | decode_text ctxt (Const (\<^const_name>\<open>type_text\<close>, _) $ \<^Const_>\<open>Pure.type T\<close>) =
+fun decode_text _ (\<^const>\<open>text.literal\<close> $ Abs (text, _, _)) = [Pretty.str (recovery_string text)]
+  | decode_text ctxt (Const (\<^const_name>\<open>text.term\<close>, _) $ x) = [Syntax.pretty_term ctxt x]
+  | decode_text ctxt (Const (\<^const_name>\<open>text.type\<close>, _) $ \<^Const_>\<open>Pure.type T\<close>) =
       [Syntax.pretty_typ ctxt T]
-  | decode_text ctxt (\<^const>\<open>cat_text\<close> $ A $ B) =
+  | decode_text ctxt (\<^const>\<open>text.cat\<close> $ A $ B) =
       decode_text ctxt A @ decode_text ctxt B
-  | decode_text ctxt (\<^const>\<open>text\<close> $ X) = decode_text ctxt X
+  | decode_text _ (\<^const>\<open>text.newline\<close>) = [Pretty.brk 0]
+  | decode_text ctxt (\<^const>\<open>text.text\<close> $ X) = decode_text ctxt X
   | decode_text _ tm = raise TERM ("decode_text", [tm])
 
-fun decode_text_str ctxt X =
-      Pretty.string_of (Pretty.block (Pretty.separate "" (decode_text ctxt X)))
+fun decode_text_pretty ctxt X = Pretty.block (Pretty.separate "" (decode_text ctxt X))
+fun decode_text_str ctxt X = Pretty.string_of (decode_text_pretty ctxt X)
 
 fun decode_text_ast ast =
   case decode_text_ast' [] ast
@@ -82,10 +91,10 @@ let open Ast
     | dest_literal (Variable x) = String.substring (x, 7, size x - 15)
         (*7 for size of \ <open> and 15 for size of \ <open> \ <close>*)
   fun encode_literal str =
-    Appl [Constant \<^const_syntax>\<open>literal_text\<close>,
+    Appl [Constant \<^const_syntax>\<open>text.literal\<close>,
     Appl [Constant \<^syntax_const>\<open>_abs\<close>,
       Appl [Constant \<^syntax_const>\<open>_constrain\<close>,
-            Variable (Encode_Text.escape_string str),
+            Variable (Text_Encoding.escape_string str),
             Constant \<^type_syntax>\<open>text\<close>],
       Appl [Constant \<^syntax_const>\<open>_constrain\<close>,
             Constant \<^const_syntax>\<open>undefined\<close>,
@@ -95,18 +104,19 @@ let open Ast
         parse (Appl [Constant \<^syntax_const>\<open>_text_term_\<close>, tm])
     | parse (Appl [Constant \<^syntax_const>\<open>_text_term_\<close>,
                        (tm as Appl [Constant \<^syntax_const>\<open>_TYPE\<close>, _])]) =
-        Appl [Constant \<^const_syntax>\<open>type_text\<close>, tm]
+        Appl [Constant \<^const_syntax>\<open>text.type\<close>, tm]
     | parse (Appl [Constant \<^syntax_const>\<open>_text_term_\<close>, tm]) =
-        Appl [Constant \<^const_syntax>\<open>term_text\<close>, tm]
+        Appl [Constant \<^const_syntax>\<open>text.term\<close>, tm]
+    | parse (Constant \<^syntax_const>\<open>_text_newline_\<close>) = Constant \<^const_syntax>\<open>text.newline\<close>
     | parse (Appl [Constant \<^syntax_const>\<open>_text_cat_\<close>, tmA, tmB]) =
-        Appl [Constant \<^const_syntax>\<open>cat_text\<close>, parse tmA, parse tmB]
+        Appl [Constant \<^const_syntax>\<open>text.cat\<close>, parse tmA, parse tmB]
 in
   [(\<^syntax_const>\<open>_text_\<close>, (fn ctxt => fn [ast] =>
-        Appl [Constant \<^const_syntax>\<open>text\<close>, parse ast]))]
+        Appl [Constant \<^const_syntax>\<open>text.text\<close>, parse ast]))]
 end\<close>
 
-print_ast_translation \<open>[(\<^const_syntax>\<open>text\<close>, (fn ctxt => fn [ast] =>
-  Ast.Appl [Ast.Constant \<^syntax_const>\<open>_text_\<close>, Encode_Text.decode_text_ast ast]))]\<close>
+print_ast_translation \<open>[(\<^const_syntax>\<open>text.text\<close>, (fn ctxt => fn [ast] =>
+  Ast.Appl [Ast.Constant \<^syntax_const>\<open>_text_\<close>, Text_Encoding.decode_text_ast ast]))]\<close>
 
 
 subsection \<open>Reasoners for Printing Message\<close>
@@ -123,7 +133,7 @@ lemma TRACING_I: \<open>TRACING x\<close>
   let
     val \<^const>\<open>Trueprop\<close> $ (\<^const>\<open>TRACING\<close> $ text)
           = Thm.major_prem_of sequent
-    val str = Encode_Text.decode_text_str ctxt text
+    val str = Text_Encoding.decode_text_str ctxt text
     val _ = tracing str
   in Seq.single (ctxt, @{thm TRACING_I} RS sequent)
   end\<close>
@@ -140,7 +150,7 @@ lemma WARNING_I: \<open>WARNING x\<close>
   let
     val \<^const>\<open>Trueprop\<close> $ (\<^const>\<open>WARNING\<close> $ text)
           = Thm.major_prem_of sequent
-    val str = Encode_Text.decode_text_str ctxt text
+    val str = Text_Encoding.decode_text_str ctxt text
     val _ = warning str
   in Seq.single (ctxt, @{thm WARNING_I} RS sequent)
   end\<close>
@@ -161,7 +171,7 @@ definition FAIL' :: \<open>text \<Rightarrow> prop\<close>
     val text = case Thm.major_prem_of sequent
                  of \<^const>\<open>Trueprop\<close> $ (\<^const>\<open>FAIL\<close> $ X) => X
                   | \<^const>\<open>FAIL'\<close> $ X => X
-    val str = Encode_Text.decode_text_str ctxt text
+    val str = Text_Encoding.decode_text_str ctxt text
     val _ = warning str
   in Seq.empty
   end\<close>
@@ -182,7 +192,7 @@ definition ERROR' :: \<open>text \<Rightarrow> prop\<close>
     val text = case Thm.major_prem_of sequent
                  of \<^const>\<open>Trueprop\<close> $ (\<^const>\<open>ERROR\<close> $ X) => X
                   | \<^const>\<open>ERROR'\<close> $ X => X
-    val str = Encode_Text.decode_text_str ctxt text
+    val str = Text_Encoding.decode_text_str ctxt text
     val _ = error str
   in Seq.empty
   end\<close>
